\documentclass{article}
\usepackage{ifthen}
\usepackage{epsfig}
\usepackage[utf8]{inputenc}
% Packages requested by user
\usepackage{amsmath}
\usepackage{amsfonts}
\usepackage{../commands}
\usepackage{newtxmath}

\usepackage{newunicodechar}
  \newunicodechar{⁻}{${}^{-}$}% Superscript minus
  \newunicodechar{²}{${}^{2}$}% Superscript two
  \newunicodechar{³}{${}^{3}$}% Superscript three

\pagestyle{empty}
\begin{document}
$\frac{1}{k^2}$
\pagebreak

$\mathcal{G}_1$
\pagebreak

$\mathcal{G}_2$
\pagebreak

\begin{eqnarray*} \mathcal{G}_1:\;& \nu_x=1,...,{\tt nx}\;,\; \nu_y=1,...,{\tt ny}\;,\; \nu_z=1,...,{\tt nz}\;;\; \\& \mbox{coordinate spacing: } {\tt dx}, {\tt dy}, {\tt dz}; \\& \mbox{momentum spacing: } {\tt dk}_x = \frac{2\pi}{{\tt nx}\!\cdot\!{\tt dx}}, {\tt dk}_y = \frac{2\pi}{{\tt ny}\!\cdot\!{\tt dy}}, {\tt dk}_z = \frac{2\pi}{{\tt nz}\!\cdot\!{\tt dz}}; \end{eqnarray*}
\pagebreak

\begin{eqnarray*} \mathcal{G}_2:\;& \nu_x=1,...,2{\tt nx}\;,\; \nu_y=1,...,2{\tt ny}\;,\; \nu_z=1,...,2{\tt nz}\;;\; \\& x_{\nu_x}=(\nu_x\!-\!{\tt nx}){\tt dx}\,,\, y_{\nu_y}=(\nu_y\!-\!{\tt ny}){\tt dy}\,,\, z_{\nu_z}=(\nu_z\!-\!{\tt nz}){\tt dz}\,; \\& \mbox{momentum spacing: } {\tt dk}_x = \frac{2\pi}{{2\tt nx}\!\cdot\!{\tt dx}}, {\tt dk}_y = \frac{2\pi}{{2\tt ny}\!\cdot\!{\tt dy}}, {\tt dk}_z = \frac{2\pi}{{2\tt nz}\!\cdot\!{\tt dz}}; \end{eqnarray*}
\pagebreak

$k_{n_i}$
\pagebreak

$k=0$
\pagebreak

${\tt dk}_i$
\pagebreak

$\mathbf{r}_{\bnu}=\left(x_{\nu_x},y_{\nu_y},z_{\nu_z}\right)$
\pagebreak

$\mathbf{k}_\mathbf{n}$
\pagebreak

\[ G(\mathbf{r}_{\bnu})=\frac{e^2}{|\mathbf{r}_{\bnu}|} \]
\pagebreak

$ 1/r $
\pagebreak

$ \vec r=0 $
\pagebreak

$\Delta x\times\Delta y\times\Delta z $
\pagebreak

$ 2.38/\Delta x $
\pagebreak

$ 2.84/\Delta x $
\pagebreak

\[ G(0) = \frac{2.84\sqrt{3}}{\sqrt{{\tt dx}^2+{\tt dy}^2+{\tt dz}^2}} \quad.\]
\pagebreak

$ k $
\pagebreak

$\tilde{G}(\mathbf{k}_{\bmu})={\tt FFT}\{G(\mathbf{r}_{\bnu})\}$
\pagebreak

$ \tilde{G}(\mathbf{k}_{\bmu}) $
\pagebreak

$ U_\mathrm{Coul}(\mathbf{r}_{\bnu}) $
\pagebreak

$\rho(\mathbf{r}_{\bnu})$
\pagebreak

$ \rho_{\bnu} $
\pagebreak

$ \mathcal{G}_1 $
\pagebreak

$ \mathcal{G}_2 $
\pagebreak

\[ \rho_2(\mathbf{r}_{\bnu}) = \left\{\begin{array}{lcl} \rho(\mathbf{r}_{\bnu}) &\mbox{ if }& 1\leq \nu_i \leq {\tt n}i \mbox{ for } i\in\{x,y,z\}\\ 0 &\mbox{ else }\end{array}\right. \]
\pagebreak

\[ \rho_2(\mathbf{r}_{\bnu})\ \longrightarrow\ \tilde{\rho}_2(\mathbf{k}_{\bmu})={\tt FFT}\{\rho_2(\mathbf{r}_{\bnu})\} \]
\pagebreak

\[ \tilde{U}_2(\mathbf{k}_{\bmu}) =\tilde{G}_2(\mathbf{k}_{\bmu})\tilde{\rho}_2(\mathbf{k}_{\bmu}) \]
\pagebreak

$ r $
\pagebreak

\[ {U}_2(\mathbf{r}_{\bnu})={\tt FFT}^{-1}\{\tilde{U}_2(\mathbf{k}_{\bmu})\} \]
\pagebreak

\[ {U}_\mathrm{Coul}(\mathbf{r}_{\bnu})=U_2(\mathbf{r}_{\bnu})\quad\mbox{for}\quad\bnu\in\mathcal{G}_1 \]
\pagebreak

$1/k^2$
\pagebreak

$1/r$
\pagebreak

$ 1/k^2 $
\pagebreak

$r^2$
\pagebreak

$k^{-2}$
\pagebreak

\[ k_i=\frac{2\pi}{n\Delta x}\bigl(0,\;1,\;2,\;\ldots \frac{n}2-1,\; -\frac{n}2,\;-\frac{n}2+1,\;\ldots -1\bigr).\]
\pagebreak

\[ d_i=d\bigl(0,\;1,\;2,\;\ldots \frac{n}2-1,\; -\frac{n}2,-\frac{n}2+1,\;\;\ldots 1\bigr).\]
\pagebreak

${\rm fm}^{-3} $
\pagebreak

\[ \rho_q(\vec r)=\sum_{k\in q}w_k^2\sum_s|\phi_k(\vec r,s)|^2,\qquad q=n,p \]
\pagebreak

\[ \tau_q(\vec r)=\sum_{k\in q}w_k^2\sum_s|\nabla\phi_k(\vec r,s)|^2, \qquad q=n,p\]
\pagebreak

$ \hbar^2/2m $
\pagebreak

\[ \vec\jmath_q(\vec r) = \frac{1}{2\I}\sum_{\alpha\in q}w_\alpha^2 \sum_s\left(\psi_\alpha^*(\vec r,s)\nabla\psi_\alpha(\vec r,s)-\psi_\alpha(\vec r,s) \nabla\psi_\alpha^*(\vec r,s)\right). \]
\pagebreak

$ \frac{\hbar}{m} $
\pagebreak

$ {\rm fm}^{-4} $
\pagebreak

\[ \vec\sigma_q(\vec r)=\sum_{\alpha\in q} w_\alpha^2 \sum_{ss'}\psi_\alpha^*(\vec r,s)\,\sigma_{ss'} \,\psi_\alpha(\vec r,s').\]
\pagebreak

$ \hbar/2 $
\pagebreak

$ {\rm fm}^{-3} $
\pagebreak

\[ \vec J_q(\vec r)=\frac{1}\I\sum_{\alpha\in q}w_\alpha^2 \sum_{ss'}\left(\psi_\alpha^*(\vec r,s)\nabla\times\sigma_{ss'} \psi_\alpha(\vec r,s')\right).\]
\pagebreak

$ w_\alpha^2= $
\pagebreak

\begin{eqnarray*} \frac{1}{2\I}(\psi^*\nabla\psi-\psi\nabla\psi^*)&=& \frac{1}{2\I}\left(\psi^*\nabla\psi-(\psi^*\nabla\psi)^*\right)\\ &=&\frac{1}{2\I}\left(2\I\Im(\psi^*\nabla\psi)\right)\\ &\rightarrow&{\tt AIMAG(CONJG(psin)*psi1)} \end{eqnarray*}
\pagebreak

$ \hat h(t+\tfrac1{2}\Delta t) $
\pagebreak

$ t $
\pagebreak

$ t+\Delta t $
\pagebreak

$ \hat h $
\pagebreak

\[ \hat U(t,t+\Delta t)\,\phi\approx \sum_{n=0}^m \phi^{(n)} \]
\pagebreak

\[ \phi^{(0)}=\phi,\qquad \phi^{(k+1)}=\frac{-\I\,\Delta t} {\hbar c k}\,\hat h\,\phi^{(k)},\quad k=0,\ldots,m-1. \]
\pagebreak

$ \hat h\phi_k $
\pagebreak

\[ E_{\rm coll}=\frac{\hbar^2}{2m}\int \D^3r \frac{{\vec \jmath\,}^2}{\rho} \]
\pagebreak

\[ \rho(\vec r) \vec k=\frac{1}{2\I}\sum_{\alpha\in q}w_\alpha^2 \sum_s\left(\psi_\alpha^*(\vec r,s)\nabla\psi_\alpha(\vec r,s)-\psi_\alpha(\vec r,s) \nabla\psi_\alpha^*(\vec r,s)\right). \]
\pagebreak

$ \exp(-\I\vec k\cdot \vec r) $
\pagebreak

$ E_{3,\rm corr} $
\pagebreak

$ E_{C,\rm corr} $
\pagebreak

$ T $
\pagebreak

\[ T=\sum_q \frac{\hbar^2}{2m_q}\int\D^3 r\, \tau_q \]
\pagebreak

$ \tau_q $
\pagebreak

$ E_0 $
\pagebreak

$ b_0 $
\pagebreak

$ b'_0 $
\pagebreak

\[ E_0=\int \D^3\!r\,\left(\frac{b_0}{2}\rho^2-\frac{b_0'}{2}\sum_q\rho_q^2\right). \]
\pagebreak

$ E_{1}$
\pagebreak

$ b_1 $
\pagebreak

$ b_1' $
\pagebreak

\[ E_1=\int \D^3\!r\,\left(b_1[\rho\tau-{\vec\jmath\,}{}^2] -b_1'\sum_q[\rho_q\tau_q-{\vec\jmath_q}{}^2]\right).\]
\pagebreak

$ E_{2} $
\pagebreak

$ b_2 $
\pagebreak

$ b_2' $
\pagebreak

\[ E_2=\int \D^3\!r\,\left(-\frac{b_2}{2}\rho\Delta\rho +\frac{b_2'}{2}\sum_q\rho_q\Delta\rho_q\right). \]
\pagebreak

$ E_{3} $
\pagebreak

\[ E_{3}=\int \D^3\!r\,\left(\frac{b_3}{3}\rho^{\alpha+2} -\frac{b_3'}{3}\rho^\alpha\sum_q\rho_q^2\right). \]
\pagebreak

$ E_\mathrm{ls} $
\pagebreak

\[ E_\mathrm{ls}=\int \D^3\!r\,\biggl( -b_4[\rho\nabla\cdot\vec J+ \vec s\cdot(\nabla\times\vec\jmath)]-b_4'\sum_q[\rho_q\nabla\cdot\vec J_q+ \vec s_q\cdot(\nabla\times\vec\jmath_q)]\biggr) \]
\pagebreak

$ E_\mathrm{C} $
\pagebreak

\[ E_\mathrm{C} = \frac{e^2}{2}\int \D^3\!r \D^3\!r' \frac{\rho_p(\vec{r})\rho_p(\vec{r'})}{|\vec{r}-\vec{r'}|} -\int \D^3\!r\,\frac{3e^2}{4}\left(\frac3{\pi}\right)^{\tfrac1{3}}\rho_p^{4/3} \]
\pagebreak

$ e $
\pagebreak

$ e^2=1.43989 $
\pagebreak

$ \cdot $
\pagebreak

$ E_\mathrm{pair} $
\pagebreak

$ \xi_q $
\pagebreak

\[ E_{\rm pair} = \frac{1}{4} \sum_{q\in\{p,n\}}V_\mathrm{pair,q} \int \D^3r |\xi_q|^2 \left[1 -\frac{\rho}{\rho_{0,\mathrm{pair}}}\right]\;. \]
\pagebreak

$ \rho_{0,\mathrm{pair}} $
\pagebreak

$ \delta $
\pagebreak

$ \rho_{0,\mathrm{pair}}\longrightarrow\infty $
\pagebreak

$ \rho_{0,\mathrm{pair}}=0.16 $
\pagebreak

$ ^{-3} $
\pagebreak

$ \hat{h}^2 $
\pagebreak

$ \hat{h}\cdot {\tt efluct}$
\pagebreak

$ \hbar $
\pagebreak

$ \vec\jmath_q{}^2 $
\pagebreak

$ \nabla\cdot\vec J_q $
\pagebreak

\[ \sum_k (\epsilon_k-\tfrac1{2}v_k)=\tfrac1{2}\sum_k(2t_k+v_k)= \tfrac1{2}\sum_k(t_k+\epsilon_k). \]
\pagebreak

\[ f(t)=\exp\left(-(t-\tau_0)^2/\Delta\tau^2\right)\cos(\omega(\tau-\tau_0)) \]
\pagebreak

\[ f(t)=\cos\left(\frac\pi{2}\left(\frac{t-\tau_0}{\Delta\tau}\right)^2\right) \theta\left(\Delta\tau-|t-\tau_0|\right)\cos(\omega(\tau-\tau_0)) \]
\pagebreak

\[ \psi_k(\vec r,s,t\!=\!0)= \psi_{k,0}(\vec r,s)\,\exp\left(-\I \eta F_q(\vec r)\right) \]
\pagebreak

$ F_q $
\pagebreak

\[ F_{1M} = (r^3 - \frac{5}{3}<r^2> r)Y_{1M} \]
\pagebreak

$ <r^2> $
\pagebreak

\[ F_{LM} = \sqrt{2L+1} r^L Y_{LM} \]
\pagebreak

$ Y_{LM} $
\pagebreak

$r_0$
\pagebreak

$\Delta_0$
\pagebreak

$ \omega $
\pagebreak

$ \Delta\tau $
\pagebreak

$ \tau_0 $
\pagebreak

$ x^2\rightarrow\sin^2\left(\pi x/x_L\right) $
\pagebreak

$ F_q(\vec r) \rightarrow \frac{F_q(\vec r)}{1+e^{(r-r_0)/\Delta r}} $
\pagebreak

$L_{val}$
\pagebreak

$Y_{L}^{M}$
\pagebreak

$M_{val}$
\pagebreak

$ Q_{zz} $
\pagebreak

\[ \sum_q\int\,\D^3r\,\rho_q(\vec r)F_q(\vec r) \]
\pagebreak

$ \frac{\hbar^2}{2m} $
\pagebreak

$ b $
\pagebreak

$ b' $
\pagebreak

$ y $
\pagebreak

$ z $
\pagebreak

$ s $
\pagebreak

$ x $
\pagebreak

$ (x,z) $
\pagebreak

$ \exp(-\I\vec k\cdot\Delta\vec r) $
\pagebreak

$ \vec k $
\pagebreak

$ 10^{-20} $
\pagebreak

$ \Delta x $
\pagebreak

\[ \exp\left(-\frac{2\pi\I k_j \Delta x}{L}\right). \]
\pagebreak

$ L={\tt nx*dx} $
\pagebreak

$ k_j $
\pagebreak

\[ T=A\frac{\hbar^2}{2m}k^2, \]
\pagebreak

$ A $
\pagebreak

$ m $
\pagebreak

\[ \frac{1}{1+\hat t/E_0} {\rm~with~} \hat t=-\frac{\hbar^2}{2m}\frac{\partial^2}{\partial x^2}. \]
\pagebreak

$ \hat t $
\pagebreak

$ B=B^{-1}A $
\pagebreak

$ 1\ldots{\tt nstmax} $
\pagebreak

\[ \sqrt{\langle\psi|\hat h^2|\psi\rangle-\langle\psi|\hat h|\psi\rangle^2}. \]
\pagebreak

\[ \sqrt{\langle\hat h\psi|\hat h\psi\rangle-\langle\psi|\hat h|\psi\rangle^2}. \]
\pagebreak

\[ \sum_s\int\D^3r\, \psi^*(\vec r,s)\psi_s(-\vec r,s). \]
\pagebreak

$ w_k^2 $
\pagebreak

$ {\rm fm}^{-1} $
\pagebreak

$ {\rm fm}^{-2} $
\pagebreak

\[\frac{\partial^2\psi}{\partial x^2}+\frac{\partial^2\psi} {\partial y^2}+\frac{\partial^2\psi} {\partial z^2}. \]
\pagebreak

\[ \frac1{E_{0\rm inv}+\hat t}\psi, \]
\pagebreak

\[ \hat t=-\frac{\hbar^2}{2m}\left(\frac{\partial^2} {\partial x^2}+\frac{\partial^2} {\partial y^2}+\frac{\partial^2}{\partial z^2}\right), \]
\pagebreak

$ U_q $
\pagebreak

$ B_q $
\pagebreak

$ \nabla\cdot\vec A_q $
\pagebreak

$ \vec A_q $
\pagebreak

$ \vec{S}_q $
\pagebreak

$ \vec W_q $
\pagebreak

$ q $
\pagebreak

$ q' $
\pagebreak

$ b_1\rho-b_1'\rho_q\longrightarrow b_1(\rho_q+\rho_{q'})-b_1'\rho_q $
\pagebreak

$ \longrightarrow $
\pagebreak

$ \alpha $
\pagebreak

$ \rho^\alpha $
\pagebreak

$ \vec J $
\pagebreak

$ \nabla\times\vec\jmath_q $
\pagebreak

\[ \hat h=U_q(\vec r)-\nabla\cdot\left[B_q(\vec r)\nabla\right] +\I\vec W_q\cdot(\vec\sigma\times\nabla) +\vec S_q\cdot\vec\sigma -\frac{\I}{2} \left[(\nabla\cdot\vec A_q)+2\vec A_q\cdot\nabla\right]. \]
\pagebreak

$ -\tfrac{\I}{2}\,\nabla\cdot\vec A_q $
\pagebreak

\[ -\frac{\partial B_q}{\partial x}\frac{\partial}{\partial x}-B_q \frac{\partial^2}{\partial x^2}, \]
\pagebreak

$ \I\vec W_q\cdot(\vec\sigma\times\nabla) $
\pagebreak

\[ (\I W_y\sigma_z-\I W_z\sigma_y)\frac{\partial}{\partial x}= \begin{pmatrix} \I W_y&-W_z\\ W_z&-\I W_y \end{pmatrix}\frac{\partial}{\partial x} \]
\pagebreak

\[ (\I W_z\sigma_x-\I W_x\sigma_z)\frac{\partial}{\partial y}= \begin{pmatrix} -\I W_x&\I W_z\\ \I W_z&\I W_x \end{pmatrix}\frac{\partial}{\partial y} \]
\pagebreak

\[ (\I W_x\sigma_y-\I W_y\sigma_x)\frac{\partial}{\partial z}= \begin{pmatrix} 0&W_x-\I W_y\\ -W_x-\I W_y & 0 \end{pmatrix}\frac{\partial}{\partial z} \]
\pagebreak

$ Q_{2m} $
\pagebreak

$ a_o $
\pagebreak

$ a_2 $
\pagebreak

$ \beta $
\pagebreak

$ \gamma $
\pagebreak

$ N $
\pagebreak

$ Z $
\pagebreak

$ \vec R_n $
\pagebreak

$ \vec R_p $
\pagebreak

$ \vec R $
\pagebreak

$ c $
\pagebreak

$ m=0 $
\pagebreak

$ Q_{20} $
\pagebreak

$ m=2 $
\pagebreak

$ Q_{22} $
\pagebreak

\[ \langle r_i^2\rangle=\frac1{A} \int \D^3r\, r_i^2\rho(\vec r). \]
\pagebreak

${\rm fm}^2 $
\pagebreak

$ a_0 $
\pagebreak

$ Q_{kl}=\int \D^3r \left(3x_kx_l-r^2\delta_{kl}\right) \rho(\vec r) $
\pagebreak

\[ Q_{20}=\sqrt{\frac{5}{16\pi}}\,Q_{zz},\qquad Q_{22}=\sqrt{\frac{5}{96\pi}}\,\left(Q_{yy}-Q_{xx}\right). \]
\pagebreak

$ \sum_k\ldots $
\pagebreak

\[ E_{\rm pair}=\frac1{2}\sum_k \Delta_k u_k v_k. \]
\pagebreak

\[ \frac{\sum_k\Delta_ku_kv_k}{\sum_k u_kv_k} \]
\pagebreak

\[ \frac{E_{\rm pair}}{\sum_k u_k v_k/2}.\]
\pagebreak

$ v_k^2\rightarrow {\tt wocc} $
\pagebreak

$ \Delta_k $
\pagebreak

$ 11.2\,{\rm MeV}/\sqrt{A} $
\pagebreak

\[ {\tt work}(\vec r)=\sum_k u_kv_k\left|\phi_k(\vec r)\right|^2 \]
\pagebreak

\[ u_kv_k=v_k\sqrt{1-v_k^2}=\sqrt{v_k^2(1-v_k^2)}=\sqrt{{\tt wocc}-{\tt wocc}^2} \]
\pagebreak

$ V_P(\vec r) $
\pagebreak

\[ V_P(\vec r)={\tt v0act}\cdot{\tt work}\cdot (1-\rho(\vec r))/{\tt rho0pr} \]
\pagebreak

$ \rho $
\pagebreak

\[ rho0pr \]
\pagebreak

\[ \Delta_k=\int\D^3r V_P(\vec r)\left|\phi_k(\vec r)\right|^2. \]
\pagebreak

$ \epsilon_F $
\pagebreak

\[ v_k^2=\frac1{2}\left(1-\frac{\epsilon_k-\epsilon_F} {\sqrt{(\epsilon_k-\epsilon_F)^2+\Delta_k^2}}\right). \]
\pagebreak

$ N=\sum_k v_k^2 $
\pagebreak

$ \pi $
\pagebreak

$ \hbar c $
\pagebreak

$ \alpha\hbar c $
\pagebreak

$ R=r_0A^{1/3} $
\pagebreak

$ x_0 $
\pagebreak

$ \rightarrow\epsilon $
\pagebreak

$ \hat h-\epsilon $
\pagebreak

\[ {\tt xnormb}=\langle {\tt psin}|{\tt ps1}\rangle=\langle {\tt psin}|\hat h|{\tt psin}\rangle\]
\pagebreak

$ \|\hat h\| $
\pagebreak

$ \epsilon $
\pagebreak

\[ {\tt exph2}=\langle {\tt psin}|\hat h^2|{\tt psin}\rangle \]
\pagebreak

\[ {\tt sp\_efluct1}=\sqrt{\|\hat h^2\|-\|\hat h\|^2} \]
\pagebreak

\[ {\tt varh2}=\|\hat h\,{\tt psin}\|^2 \]
\pagebreak

\[ {\tt sp\_efluct2}=\sqrt{\|\hat h\,{\tt psin}\|^2/\|{\tt psin}\|^2-\|\hat h\|^2}. \]
\pagebreak

\[ |{\tt ps1}\rangle-{\tt xnormb}\,|{\tt psin}\rangle=\left(\hat h -\langle {\tt psin}|\hat h|{\tt psin}\rangle\right)\,|{\tt psin}\rangle \]
\pagebreak

\[ \frac{x_{0\rm dmp}}{E_{0\rm inv}+\hat t}\,|{\tt ps1}\rangle. \]
\pagebreak

\[ |\psi|=\sum_{s=\pm{1\over2}}\int |\psi(\vec r,s)|^2\,\D^3 r\rightarrow {\tt wxyz}\sum_{s=1}^2 \sum_{i=1}^{nx}\sum_{j=1}^{ny}\sum_{k=1}^{nz} |{\tt psi(i,j,k,s)}|^2, \]
\pagebreak

$ psi_L $
\pagebreak

$ psi_R $
\pagebreak

\begin{eqnarray} \langle\psi_L|\psi_R\rangle&=&\sum_{s=\pm{1\over2}}\int \psi_L^*(\vec r)\,\psi_R(\vec r)\,\D^3 r \\ &\rightarrow& {\tt wxyz}\sum_{s=1}^2 \sum_{i=1}^{nx}\sum_{j=1}^{ny}\sum_{k=1}^{nz} {\tt CONJG(pl(i,j,k,s))pr(i,j,k,s)}. \end{eqnarray}
\pagebreak

$^{-4}$
\pagebreak

$c$
\pagebreak

$\Theta$
\pagebreak

$\vec L=\Theta\vec\omega$
\pagebreak

\[r(\phi)=\frac{k}{\epsilon\cos\phi-1}.\]
\pagebreak

$r$
\pagebreak

$\phi$
\pagebreak

$-\phi_\infty<\phi<\phi_\infty$
\pagebreak

$\phi_\infty=\cos^{-1}(\epsilon^{-1})$
\pagebreak

$\phi=0$
\pagebreak

$x$
\pagebreak

$z$
\pagebreak

$k$
\pagebreak

$\epsilon$
\pagebreak

$E_{\rm cm}$
\pagebreak

$b$
\pagebreak

$\vec r_{0i},\;i=1,2$
\pagebreak

$A_i$
\pagebreak

$Z_i$
\pagebreak

\[\vec r(t=0)=\vec r_2(t=0)-\vec r_1(t=0),\]
\pagebreak

\[\mu=m_0\frac{A_1A_2}{A_1+A_2},\]
\pagebreak

\[L_{\rm init}=\mu v_{\rm init}b=\mu\sqrt{\frac{2E_{\rm cm}}{\mu}}\, \frac{b}{\hbar}.\]
\pagebreak

\[ k=\frac{L_{\rm init}^2\hbar^2}{e^2Z_1Z_2\mu},\]
\pagebreak

\[a=\frac{e^2Z_1Z_2}{2E_{\rm cm}},\]
\pagebreak

\[\epsilon=\frac{\sqrt{a^2+b^2}}{a}.\]
\pagebreak

\[\phi_\infty=\cos^{-1}(1/\epsilon)\]
\pagebreak

\[\phi(t=0)=\cos^{-1}\left(\frac{k/|\vec r(t=0)|+1}{\epsilon}\right).\]
\pagebreak

\[\phi_{\rm incoming}=\phi_\infty-\phi(t=0).\]
\pagebreak

$y$
\pagebreak

$x-z $
\pagebreak

$(x,z)$
\pagebreak

\[(q_{11}-\lambda)(q_{33}-\lambda)-q_{13}^2=0,\]
\pagebreak

$\lambda$
\pagebreak

\[\lambda=\frac1{2}\left(q_{11}+q_{33}+\sqrt{(q_{11}-q_{33})^2 -4q_{13}^2}\right),\]
\pagebreak

$q_{13}x+(q_{33}-\lambda)z=0$
\pagebreak

\begin{eqnarray*} z&=&\frac{q_{13}}{\lambda-q_{33}}\,x\\ &=& \frac{q_{13}}{\frac1{2}\left(q_{11}-q_{33}+\sqrt{(q_{11}-q_{33})^2 -4q_{13}^2}\right)}. \end{eqnarray*}
\pagebreak

\end{document}
